rework repl_fun again, and push the proofs further
The problem was that the initial bytecode should not be run, it should
just be there. So, now we don't start the REPL with empty_bc_state but
rather with (strip_labels initial_bc_state). (This is better than the
alternative of having the main loop check whether it's in the initial
case every time before deciding whether to run the code.)

Also, fixed some mistakes in the definition of main_loop after the
unrolled stage, and prove the unrolled version correct. The statement
mentions the output from running the basis program - somewhere we will
have to prove that that is empty...

repl/repl_funScript.sml
@@ -83,7 +83,7 @@ val simple_main_loop_def = tDefine "simple_main_loop" `
            | SOME (Stop success) =>
              let new_s = if success then s' else s_exc in
              let (res,assert) = simple_main_loop (new_bs,new_s) rest_of_input in
-               (Result (new_bs.output) res, assert /\ code_assert)
+               (Result (new_bs.output) res, code_assert /\ assert)
            | _ => (ARB,F)))
      | Failure error_msg =>
          let (res,assert) = simple_main_loop (bs,s) rest_of_input in
@@ -105,15 +105,13 @@ val simple_repl_fun_def = Define `
 (* The remainder of the file makes definitions of a REPL function that get
    progressively closer to a specification suitable for implementation in
    machine-code. The first step is unrolling the first iteration of the loop,
-   and packaging up iterations in a function called repl_step. The first
-   iteration also installs the code in initial_bc_state, so that
-   unrolled_repl_fun can start with the empty_bc_state. *)
+   and packaging up iterations in a function called repl_step. *)
 
 val labelled_repl_step_def = Define `
   labelled_repl_step state =
     case state of
     | INL (initial,code) => (* first time around *)
-       INL (code ++ REVERSE initial_bc_state.code,initial,initial)
+       INL (code,initial,initial)
     | INR (tokens,success,s,s_exc) => (* received some input *)
         let s = if success then s else s_exc in
         case parse_infertype_compile tokens s of
@@ -141,16 +139,16 @@ val unrolled_main_loop_def = tDefine "unrolled_main_loop" `
       | SOME new_bs =>
           let success = (bc_fetch new_bs = SOME (Stop T)) in
             case lex_until_toplevel_semicolon input of
-             | NONE => (Terminate,code_assert)
+             | NONE => (Result new_bs.output Terminate,code_assert)
              | SOME (ts,rest) =>
                let (res,assert) =
                  unrolled_main_loop (INR (ts,success,new_states)) new_bs rest in
-                 (res, code_assert ∧ assert)`
+                 (Result new_bs.output res, code_assert ∧ assert)`
   tac;
 
 val unrolled_repl_fun_def = Define `
   unrolled_repl_fun initial input =
-    unrolled_main_loop (INL initial) empty_bc_state input`
+    unrolled_main_loop (INL initial) initial_bc_state input`
 
 (* The next step does label removal and moves to more concrete types, in
    particular bytecode instructions are encoded as numbers and tokens are
@@ -159,10 +157,10 @@ val unrolled_repl_fun_def = Define `
 val unlabelled_repl_step_def = Define `
   unlabelled_repl_step state =
     case state of
-    | INL (initial,code) =>
-       let code = initial_bc_state.code ++ REVERSE code in
-       let labs = collect_labels code 0 real_inst_length in
-       let len = code_length real_inst_length code in
+    | INL (len,labs,(initial,code)) =>
+       let code = REVERSE code in
+       let labs = FUNION labs (collect_labels code len real_inst_length) in
+       let len = len + code_length real_inst_length code in
        let code = inst_labels labs code in
        INL (MAP bc_num code,len,labs,initial,initial)
     | INR (symbols,success,len,labs,s,s_exc) =>
@@ -200,16 +198,19 @@ val unlabelled_main_loop_def = tDefine "unlabelled_main_loop" `
       | SOME new_bs =>
           let success = (bc_fetch new_bs = SOME (Stop T)) in
             case lex_until_top_semicolon_alt input of
-             | NONE => (Terminate,code_assert)
+             | NONE => (Result new_bs.output Terminate,code_assert)
              | SOME (syms,rest) =>
                  let (res,assert) =
                    (unlabelled_main_loop (INR (syms,success,new_states)) new_bs rest)
-                 in (res, code_assert ∧ assert)`
+                 in (Result new_bs.output res, code_assert ∧ assert)`
   tac;
 
 val unlabelled_repl_fun_def = Define`
   unlabelled_repl_fun initial input =
-    unlabelled_main_loop (INL initial) empty_bc_state input`
+    let code = REVERSE initial_bc_state.code in
+    let labs = collect_labels code 0 real_inst_length in
+    let len = code_length real_inst_length code in
+    unlabelled_main_loop (INL (len,labs,initial)) (strip_labels initial_bc_state) input`
 
 (* The last step introduces the actual initial repl state (obtained by running
    the semantics on the initial program). *)
@@ -224,7 +225,10 @@ val basis_state_def = Define`
                                  e.inf_tenvC,
                                  e.inf_tenvE);
            rcompiler_state := e.comp_rs |> in
-  (rf,Stop T :: SND (THE basis_env) ++ SND (THE prim_env))`
+  let code = REVERSE initial_bc_state.code in
+  let labs = collect_labels code 0 real_inst_length in
+  let len = code_length real_inst_length code in
+  (len,labs,(rf,Stop T :: SND (THE basis_env) ++ SND (THE prim_env)))`
 
 val basis_repl_step_def = Define `
   (basis_repl_step NONE = unlabelled_repl_step (INL basis_state)) ∧
@@ -250,16 +254,16 @@ val basis_main_loop_def = tDefine "basis_main_loop" `
       | SOME new_bs =>
           let success = (bc_fetch new_bs = SOME (Stop T)) in
             case lex_until_top_semicolon_alt input of
-             | NONE => (Terminate,code_assert)
+             | NONE => (Result new_bs.output Terminate,code_assert)
              | SOME (syms,rest) =>
                  let (res,assert) =
                    basis_main_loop (SOME (syms,success,new_states)) new_bs rest
-                 in (res, assert ∧ code_assert)`
+                 in (Result new_bs.output res, code_assert ∧ assert)`
   tac;
 
 val basis_repl_fun_def = Define`
   basis_repl_fun input =
-    basis_main_loop NONE empty_bc_state input`
+    basis_main_loop NONE (strip_labels initial_bc_state) input`
 
 val basis_repl_env_def = Define`
   basis_repl_env =
